src/arch/x64/X64.Vale.Memtaint_i.fst
@@ -1,8 +1,0 @@
-module X64.Vale.Memtaint_i
-open X64.Machine_s
-open X64.Memory_i
-open FStar.FunctionalExtensionality
-
-let equal memtaint1 memtaint2 = feq memtaint1 memtaint2
-let lemma_equal_intro memtaint1 memtaint2 = ()
-let lemma_equal_elim memtaint1 memtaint2 = ()
