src/arch/x64/X64.Vale.StateLemmas_i.fsti
@@ -7,8 +7,6 @@ module M = TransparentMap
 module BS = X64.Bytes_Semantics_s
 module ME = X64.Memory_i_s
 module TS = X64.Taint_Semantics_s
-module MT = X64.Vale.Memtaint_i
-open Taint_interop
 
 unfold let ok' s = s.ME.state.BS.ok
 unfold let regs' s = s.ME.state.BS.regs
@@ -47,11 +45,11 @@ val lemma_to_trace : s:state -> Lemma
   [SMTPat s.trace]
 
 val lemma_to_memTaint : s:state -> Lemma
-  (ensures s.memTaint == up_taint (memTaint' (state_to_S s)) s.mem)
+  (ensures s.memTaint == ME.up_taint (memTaint' (state_to_S s)) s.mem)
   [SMTPat s.memTaint]
 
 val lemma_to_memTaint2 : s:state -> Lemma
-  (ensures down_taint s.memTaint s.mem == memTaint' (state_to_S s))
+  (ensures ME.down_taint s.memTaint s.mem == memTaint' (state_to_S s))
   [SMTPat s.memTaint]
 
 val lemma_to_eval_operand : s:state -> o:operand -> Lemma
@@ -77,39 +75,39 @@ val lemma_to_of : s:TS.traceState -> Lemma
 unfold let op_String_Access (#a:eqtype) (#b:Type) (x:Map.t a b) (y:a) : Tot b = Map.sel x y
 
 val lemma_valid_taint64: (b:X64.Memory_i.buffer64) ->
-			 (memTaint:MT.t) ->
+			 (memTaint:X64.Memory_i.memtaint) ->
 			 (mem:X64.Memory_i.mem) ->
 			 (i:nat{i < X64.Memory_i.buffer_length b}) ->
 			 (t:taint) -> Lemma
-  (requires valid_taint_buf64 b memTaint t)
-  (ensures (down_taint memTaint mem).[X64.Memory_i.buffer_addr b mem + 8 `op_Multiply` i] == t)
+  (requires X64.Memory_i.valid_taint_buf64 b memTaint t)
+  (ensures (ME.down_taint memTaint mem).[X64.Memory_i.buffer_addr b mem + 8 `op_Multiply` i] == t)
 
 val lemma_valid_taint128: (b:X64.Memory_i.buffer128) ->
-			 (memTaint:MT.t) ->
+			 (memTaint:X64.Memory_i.memtaint) ->
 			 (mem:X64.Memory_i.mem) ->
 			 (i:nat{i < X64.Memory_i.buffer_length b}) ->
 			 (t:taint) -> Lemma
-  (requires valid_taint_buf128 b memTaint t)
-  (ensures (down_taint memTaint mem).[X64.Memory_i.buffer_addr b mem + 16 `op_Multiply` i] == t)
+  (requires X64.Memory_i.valid_taint_buf128 b memTaint t)
+  (ensures (ME.down_taint memTaint mem).[X64.Memory_i.buffer_addr b mem + 16 `op_Multiply` i] == t)
 
 
 val modify_trace: (s0:state) -> (b:bool) -> Lemma
   (state_to_S ({s0 with trace=BranchPredicate(b)::s0.trace}) == ({(state_to_S s0) with TS.trace = BranchPredicate(b)::(state_to_S s0).TS.trace}))
 
-val same_memTaint: (b:X64.Memory_i.buffer64) -> 
+val same_memTaint64: (b:X64.Memory_i.buffer64) -> 
                    (mem0:X64.Memory_i.mem) ->
 		   (mem1:X64.Memory_i.mem) ->
-		   (memtaint0:MT.t) ->
-		   (memtaint1:MT.t) -> Lemma
+		   (memtaint0:X64.Memory_i.memtaint) ->
+		   (memtaint1:X64.Memory_i.memtaint) -> Lemma
   (requires (X64.Memory_i.modifies (X64.Memory_i.loc_buffer b) mem0 mem1 /\ 
-    (forall p. Map.sel (down_taint memtaint0 mem0) p == Map.sel (down_taint memtaint1 mem1) p)))
+    (forall p. Map.sel (ME.down_taint memtaint0 mem0) p == Map.sel (ME.down_taint memtaint1 mem1) p)))
   (ensures memtaint0 == memtaint1)
 
 val same_memTaint128: (b:X64.Memory_i.buffer128) -> 
                    (mem0:X64.Memory_i.mem) ->
 		   (mem1:X64.Memory_i.mem) ->
-		   (memtaint0:MT.t) ->
-		   (memtaint1:MT.t) -> Lemma
+		   (memtaint0:X64.Memory_i.memtaint) ->
+		   (memtaint1:X64.Memory_i.memtaint) -> Lemma
   (requires (X64.Memory_i.modifies (X64.Memory_i.loc_buffer b) mem0 mem1 /\ 
-    (forall p. Map.sel (down_taint memtaint0 mem0) p == Map.sel (down_taint memtaint1 mem1) p)))
+    (forall p. Map.sel (ME.down_taint memtaint0 mem0) p == Map.sel (ME.down_taint memtaint1 mem1) p)))
   (ensures memtaint0 == memtaint1)
